veric/composite_compute.v
@@ -2,6 +2,43 @@ Require Import Coq.Sorting.Permutation.
 Require Import VST.veric.base.
 Require Import VST.veric.Clight_lemmas.
 
+Lemma PTree_In_fst_elements {A: Type}: forall (T: PTree.t A) i,
+  In i (map fst (PTree.elements T)) <-> exists a, PTree.get i T = Some a.
+Proof.
+  intros.
+  split; intros.
+  + apply list_in_map_inv in H.
+    destruct H as [[i0 a] [? ?]].
+    simpl in H; subst i0.
+    apply PTree.elements_complete in H0.
+    eauto.
+  + destruct H as [a ?].
+    apply PTree.elements_correct in H.
+    apply (in_map fst) in H.
+    auto.
+Qed.
+
+Lemma PTree_gs {A: Type}: forall (T: PTree.t A) i j x,
+  (exists a, PTree.get i T= Some a) ->
+  exists a, PTree.get i (PTree.set j x T) = Some a.
+Proof.
+  intros.
+  destruct H.
+  destruct (Pos.eq_dec i j).
+  + subst.
+    rewrite PTree.gss; eauto.
+  + rewrite PTree.gso; eauto.
+Qed.
+
+Lemma PTree_set_In_fst_elements {A: Type}: forall (T: PTree.t A) i i' a',
+  In i (map fst (PTree.elements T)) ->
+  In i (map fst (PTree.elements (PTree.set i' a' T))).
+Proof.
+  intros.
+  rewrite PTree_In_fst_elements in H |- *.
+  apply PTree_gs; auto.
+Qed.
+  
 Fixpoint relative_defined_type {A: Type} (l: list (ident * A)) (t: type): Prop :=
   match t with
   | Tarray t' _ _ => relative_defined_type l t'
@@ -9,6 +46,49 @@ Fixpoint relative_defined_type {A: Type} (l: list (ident * A)) (t: type): Prop :
   | Tunion id _ => In id (map fst l)
   | _ => True
   end.
+
+(* Aux: composite_env's PTree members reordering *)
+
+Definition PTree_get_list {A: Type} (i: positive) (T: PTree.t (list A)): list A :=
+  match PTree.get i T with
+  | Some l => l
+  | None => nil
+  end.
+
+Definition PTree_set_cons {A: Type} (i: positive) (a: A) (T: PTree.t (list A)) :=
+  PTree.set i (a :: PTree_get_list i T) T.
+
+Definition rebuild_composite_tree (env: composite_env): PTree.t (list (ident * composite)) :=
+  fold_right (fun ic => PTree_set_cons (Pos.of_succ_nat (co_rank (snd ic))) ic) (PTree.empty _) (PTree.elements env).
+
+Definition max_rank_composite (env: composite_env): nat :=
+  fold_right (fun ic => max (co_rank (snd ic))) O (PTree.elements env).
+
+Lemma max_rank_composite_is_upper_bound: forall env i co,
+  PTree.get i env = Some co ->
+  (co_rank co <= max_rank_composite env)%nat.
+Proof.
+  intros.
+  apply PTree.elements_correct in H.
+  unfold max_rank_composite.
+  induction (PTree.elements env).
+  + inv H.
+  + destruct H.
+    - subst.
+      simpl.
+      apply Max.le_max_l.
+    - apply IHl in H.
+      etransitivity; [exact H |].
+      simpl.
+      apply Max.le_max_r.
+Qed.
+
+Inductive ordered_composite: list (positive * composite) -> Prop :=
+| ordered_composite_nil: ordered_composite nil
+| ordered_composite_cons: forall i co l,
+    Forall (relative_defined_type l) (map snd (co_members co)) ->
+    ordered_composite l ->
+    ordered_composite ((i, co) :: l).
 
 Module type_func.
 Section type_func.
@@ -36,31 +116,154 @@ Fixpoint F (env: PTree.t A) (t: type): A :=
   | _ => f_default t
   end.
 
-Fixpoint Env (l: list (positive * composite)): PTree.t A :=
-  fold_right
-    (fun (ic: positive * composite) env =>
-       let (i, co) := ic in
-       PTree.set i
-                 (f_member (co_su co)
-                           (map
-                              (fun it0: positive * type =>
-                                 let (i0, t0) := it0 in (i0, F env t0))
-                              (co_members co)))
-                 env)
-    (PTree.empty A)
-    l.
+Definition Completeness (cenv: composite_env) (env: PTree.t A): Prop :=
+  forall i co,
+    PTree.get i cenv = Some co ->
+    exists a, PTree.get i env = Some a.
 
-Lemma Consistent: forall env l,
-  Permutation l (PTree.elements env) ->
-  (forall l1 i co l2,
-      l = l1 ++ (i, co) :: l2 ->
-      Forall (relative_defined_type l1) (map snd (co_members co))) ->
+Definition Consistency (cenv: composite_env) (env: PTree.t A): Prop :=
   forall i co a,
-    PTree.get i env = Some co ->
-    PTree.get i (Env (PTree.elements env)) = Some a ->
+    PTree.get i cenv = Some co ->
+    PTree.get i env = Some a ->
     a = f_member (co_su co) (map
                               (fun it0: positive * type =>
                                  let (i0, t0) := it0 in
-                                 (i0, F (Env l) t0))
+                                 (i0, F env t0))
                               (co_members co)).
-                 .
+
+Definition env_rec (i: positive) (co: composite) (env: PTree.t A): PTree.t A :=
+  PTree.set i
+    (f_member (co_su co) (map
+                              (fun it0: positive * type =>
+                                 let (i0, t0) := it0 in (i0, F env t0))
+                              (co_members co)))
+    env.
+
+Fixpoint Env (l: list (positive * composite)): PTree.t A :=
+  fold_right
+    (fun (ic: positive * composite) =>
+       let (i, co) := ic in env_rec i co)
+    (PTree.empty A)
+    l.
+
+Lemma F_PTree_set: forall t env i a,
+  ~ In i (map fst (PTree.elements env)) ->
+  relative_defined_type (PTree.elements env) t ->
+  F env t = F (PTree.set i a env) t.
+Proof.
+  intros.
+  induction t; auto.
+  + simpl.
+    apply IHt in H0.
+    rewrite H0; auto.
+  + simpl in H0 |- *.
+    rewrite PTree.gso; auto.
+    intro; subst; tauto.
+  + simpl in H0 |- *.
+    rewrite PTree.gso; auto.
+    intro; subst; tauto.
+Qed.    
+
+Lemma relative_defined_type_PTree_set: forall t (env: PTree.t A) i a,
+  relative_defined_type (PTree.elements env) t ->
+  relative_defined_type (PTree.elements (PTree.set i a env)) t.
+Proof.
+  intros.
+  induction t; auto.
+  + simpl in H |- *.
+    apply PTree_set_In_fst_elements; auto.
+  + simpl in H |- *.
+    apply PTree_set_In_fst_elements; auto.
+Qed.
+
+Lemma aux_induction_step: forall cenv env i0 co0,
+  ~ In i0 (map fst (PTree.elements env)) ->
+  Forall (relative_defined_type (PTree.elements env)) (map snd (co_members co0)) ->
+  PTree.get i0 cenv = Some co0 ->
+  (forall i co a,
+      PTree.get i cenv = Some co ->
+      PTree.get i env = Some a ->
+      Forall (relative_defined_type (PTree.elements env)) (map snd (co_members co))) ->
+  (forall i co a,
+      PTree.get i cenv = Some co ->
+      PTree.get i (env_rec i0 co0 env) = Some a ->
+      Forall (relative_defined_type (PTree.elements (env_rec i0 co0 env))) (map snd (co_members co))).
+Proof.
+  intros ? ? i0 co0 NOT_IN RDT CENV0 IH_RDT.
+  intros i co a CENV ENV.
+  unfold env_rec in ENV.
+  destruct (Pos.eq_dec i i0).
+  + subst i0; rewrite CENV in CENV0; inversion CENV0; subst co0; clear CENV0.
+    rewrite PTree.gss in ENV.
+    inversion ENV; clear a ENV H0.
+    revert RDT.
+    apply Forall_impl; intros t.
+    apply relative_defined_type_PTree_set.
+  + rewrite PTree.gso in ENV by auto.
+    specialize (IH_RDT _ _ _ CENV ENV).
+    revert IH_RDT.
+    apply Forall_impl; intros t.
+    apply relative_defined_type_PTree_set.
+Qed.
+
+Lemma consistent_induction_step: forall cenv env i0 co0,
+  ~ In i0 (map fst (PTree.elements env)) ->
+  Forall (relative_defined_type (PTree.elements env)) (map snd (co_members co0)) ->
+  PTree.get i0 cenv = Some co0 ->
+  (forall i co a,
+      PTree.get i cenv = Some co ->
+      PTree.get i env = Some a ->
+      Forall (relative_defined_type (PTree.elements env)) (map snd (co_members co))) ->
+  Consistency cenv env ->
+  Consistency cenv (env_rec i0 co0 env).
+Proof.
+  intros ? ? i0 co0 NOT_IN RDT CENV0 IH_RDT IH_main.
+  intros i co a CENV ENV.
+  unfold env_rec in ENV.
+  destruct (Pos.eq_dec i i0).
+  + subst i0; rewrite CENV in CENV0; inversion CENV0; subst co0; clear CENV0.
+    rewrite PTree.gss in ENV.
+    inversion ENV; clear a ENV H0.
+    f_equal.
+    auto.
+    apply map_ext_in.
+    intros (i1, t1) ?.
+    f_equal.
+    apply F_PTree_set; auto.
+    rewrite Forall_forall in RDT; apply RDT.
+    apply (in_map snd) in H; auto.
+  + rewrite PTree.gso in ENV by auto.
+    specialize (IH_main _ _ _ CENV ENV).
+    subst a.
+    f_equal.
+    apply map_ext_in.
+    intros (i1, t1) ?.
+    f_equal.
+    apply F_PTree_set; auto.
+    specialize (IH_RDT _ _ _ CENV ENV).
+    rewrite Forall_forall in IH_RDT; apply IH_RDT.
+    apply (in_map snd) in H; auto.
+Qed.
+
+Lemma Consistent: forall cenv l,
+  Permutation l (PTree.elements cenv) ->
+  ordered_composite l ->
+  Consistency cenv (Env l).
+Proof.
+  intros.
+  assert (
+    (forall i co a,
+      PTree.get i cenv = Some co ->
+      PTree.get i (Env l) = Some a ->
+      Forall (relative_defined_type (PTree.elements (Env l))) (map snd (co_members co))) /\
+    Consistency cenv (Env l)); [| tauto].
+  induction l as [| [i0 co0] l].
+  + split; hnf; intros.
+    - unfold Env in H2; simpl in H2.
+      rewrite PTree.gempty in H2; inv H2.
+    - unfold Env in H2; simpl in H2.
+      rewrite PTree.gempty in H2; inv H2.
+  + split.
+    - apply aux_induction_step; admit.
+    - apply consistent_induction_step; admit.
+Admitted.
